theories/tree_valid_state.v
@@ -60,26 +60,26 @@ Module B.
       by rewrite base_and_big_and in bA.
     Qed.
 
-    Lemma base_or_aux_big_or_aux s l:
-      base_or_aux (big_or_aux s l).
+    Lemma base_or_aux_big_or s l:
+      base_or_aux (big_or s l).
     Proof.
       elim: l s => //=; clear.
       + by case => //= _ l; rewrite eqxx base_and_big_and.
       + by move=> [s r] rs IH r1 /=; rewrite IH base_and_big_and.
     Qed.
 
-    Lemma bbOr_big_or_aux s l: bbOr (big_or_aux s l).
+    Lemma bbOr_big_or s l: bbOr (big_or s l).
     Proof.
       rewrite/bbOr.
-      case: base_or_aux_ko; rewrite ?orbT//orbF base_or_aux_big_or_aux//.
+      case: base_or_aux_ko; rewrite ?orbT//orbF base_or_aux_big_or//.
     Qed.
 
     Lemma spec_base_or_aux A:
-      reflect (exists X Y, big_or_aux X Y = A) (base_or_aux A).
+      reflect (exists X Y, big_or X Y = A) (base_or_aux A).
     Proof.
       case bA: base_or_aux; constructor; last first.
         move=> [X[Y H]]; subst.
-        by rewrite base_or_aux_big_or_aux in bA.
+        by rewrite base_or_aux_big_or in bA.
       pose head := RCallable_Kp (IKp 1).
       elim: A bA => //=; first by exists [::],[::].
         move=> A _ s B HB /andP[/spec_base_and[L <-]] /HB [X [Y <-]].
@@ -112,11 +112,11 @@ Module B.
     Qed.
 
     Lemma spec_base_or_aux_ko A:
-      reflect (exists X Y, cutr (big_or_aux X Y) = A) (base_or_aux_ko A).
+      reflect (exists X Y, cutr (big_or X Y) = A) (base_or_aux_ko A).
     Proof.
       case bA: base_or_aux_ko; constructor; last first.
         move=> [X[Y H]]; subst.
-        by rewrite base_or_base_or_ko_cutr//base_or_aux_big_or_aux in bA.
+        by rewrite base_or_base_or_ko_cutr//base_or_aux_big_or in bA.
       pose head := RCallable_Kp (IKp 1).
       elim: A bA => //=; first by exists [::],[::].
         move=> A _ s B HB /andP[/spec_base_and_ko[X?]] /HB [Y[Z H]]; subst.
@@ -145,12 +145,12 @@ Module B.
 End B.
 
 Lemma spec_bbOr A:
-  reflect (exists X Y, let x := (big_or_aux X Y) in x = A \/ cutr x = A) (B.bbOr A).
+  reflect (exists X Y, let x := (big_or X Y) in x = A \/ cutr x = A) (B.bbOr A).
 Proof.
   case X: B.bbOr; constructor.
     move/orP: X => [/B.spec_base_or_aux|/B.spec_base_or_aux_ko][?[??]]/=; subst; repeat eexists; eauto.
   move=> [Y [Z]]/=[]?; subst;
-  by rewrite !(B.bbOr_cutr,B.bbOr_big_or_aux) in X.
+  by rewrite !(B.bbOr_cutr,B.bbOr_big_or) in X.
 Qed.
 
 (*BEGIN*)
@@ -194,33 +194,33 @@ Section valid_tree.
   Lemma valid_tree_big_and_cutr l : valid_tree (cutr (big_and l)).
   Proof. elim: l => //=. Qed.
 
-  Lemma valid_tree_big_or_aux s l : valid_tree (big_or_aux s l).
+  Lemma valid_tree_big_or s l : valid_tree (big_or s l).
   Proof.
     elim: l s => [|[]] //=.
     + move=> s; rewrite valid_tree_big_and//.
-    + by move=> _ b l H s; rewrite is_dead_big_and valid_tree_big_and B.bbOr_big_or_aux.
+    + by move=> _ b l H s; rewrite is_dead_big_and valid_tree_big_and B.bbOr_big_or.
   Qed.
 
-  Lemma valid_tree_big_or_aux_cutr s l : valid_tree (cutr (big_or_aux s l)).
+  Lemma valid_tree_big_or_cutr s l : valid_tree (cutr (big_or s l)).
   Proof.
     elim: l s => [|[]] //=.
     + by move=> s; rewrite valid_tree_big_and_cutr.
-    + by move=> _ r l IH s; rewrite IH valid_tree_big_and_cutr B.bbOr_cutr (if_same, B.bbOr_big_or_aux).
+    + by move=> _ r l IH s; rewrite IH valid_tree_big_and_cutr B.bbOr_cutr (if_same, B.bbOr_big_or).
   Qed.
 
 
-  Lemma valid_tree_big_or {pr s t} : valid_tree (big_or u pr s t).
+  Lemma valid_tree_backchain {pr s t} : valid_tree (backchain u pr s t).
   Proof.
-    rewrite/big_or; case: F => //[[s1 r1] rs]/=.
-    apply: B.bbOr_big_or_aux.
+    rewrite/backchain; case: F => //[[s1 r1] rs]/=.
+    apply: B.bbOr_big_or.
   Qed.
 
   Lemma bbOr_valid {B}:
     B.bbOr B -> valid_tree B.
   Proof.
     move=> /spec_bbOr[X[Y /=[]<-]].
-      apply: valid_tree_big_or_aux.
-    apply: valid_tree_big_or_aux_cutr.
+      apply: valid_tree_big_or.
+    apply: valid_tree_big_or_cutr.
   Qed.
 
   Lemma valid_tree_cut {A}: success A -> valid_tree A -> valid_tree (cutl A).
@@ -240,7 +240,7 @@ Section valid_tree.
   Proof.
     move=>+<-; clear r.
     elim: A s => //; try by move=> s r // *; subst.
-    + by move=> /= []//=>; rewrite valid_tree_big_or.
+    + by move=> /= []//=>; rewrite valid_tree_backchain.
     + move=> A IHA s B IHB s1/=.
       case:ifP => //[dA vB|dA/andP[vA bB]]/=.
         by rewrite IHB//dA.
